core/theories/Specification.v
@@ -2,7 +2,7 @@
  * Copyright (C) 2018–2019 ANSSI
  *
  * Contributors:
- * 2018 Thomas Letan <thomas.letan@ssi.gouv.fr>
+ * 2018–2019 Thomas Letan <thomas.letan@ssi.gouv.fr>
  *
  * This program is free software: you can redistribute it and/or modify
  * it under the terms of the GNU General Public License as published by
@@ -18,18 +18,190 @@
  * along with this program. If not, see <http://www.gnu.org/licenses/>.
  *)
 
-(* begin hide *)
 Require Import Coq.Program.Basics.
 Require Import Coq.Program.Equality.
 Require Import Coq.Setoids.Setoid.
 Require Import Coq.Logic.Classical.
-(* end hide *)
+
+Require Import Prelude.Equality.
 
 Require Import FreeSpec.Program.
 Require Import FreeSpec.Semantics.
-Require Import FreeSpec.Abstract.
 
-(** * Abstract Specification Definition
+(** In this library, we provide an alternative to [runProgram] we can
+    use to derive a so-called abstract state through the executed
+    effects of the underlying [Interface]. Using this feature, we can
+    verify some properties of a given [Program] _without modifying
+    it_. *)
+
+(** * Witness State and Instrumented Execution *)
+
+Section def.
+Variables (W: Type)
+          (I: Interface)
+          (abs_step:  forall (R:Type), I R -> R -> W -> W).
+
+Fixpoint runInstrumentedProgram
+         {A:         Type}
+         (w:         W)
+         (sig:       Sem.t I)
+         (p:         Program I A)
+  : Sem.result I (A * W) :=
+  match p with
+  | Pure a
+    => Sem.mkRes (a, w) sig
+  | Request e f
+    => runInstrumentedProgram
+         (abs_step _ e (evalEffect sig e) w)
+         (execEffect sig e)
+         (f (evalEffect sig e))
+  end.
+
+Lemma runInstrumentedProgram_equation_2
+      {A B: Type}
+      (w: W)
+      (sig: Sem.t I)
+      (e: I A)
+      (f: A -> Program I B)
+  : runInstrumentedProgram w sig (Request e f)
+    = runInstrumentedProgram
+        (abs_step _ e (evalEffect sig e) w)
+        (execEffect sig e)
+        (f (evalEffect sig e)).
+Proof.
+  reflexivity.
+Qed.
+
+(** Similary to [FreeSpec.Program.runProgram], we define several
+    helpers functions to select one element among the three that are
+    returned by [abstractRun].
+ *)
+Definition execInstrumentedProgram
+           {A:         Type}
+           (w:         W)
+           (sig:       Sem.t I)
+           (p:         Program I A)
+  : Sem.t I :=
+  Sem.next (runInstrumentedProgram w sig p).
+
+Lemma execInstrumentedProgram_equation_2
+      {A B: Type}
+      (w: W)
+      (sig: Sem.t I)
+      (e: I A)
+      (f: A -> Program I B)
+  : execInstrumentedProgram w sig (Request e f)
+    = execInstrumentedProgram
+        (abs_step _ e (evalEffect sig e) w)
+        (execEffect sig e)
+        (f (evalEffect sig e)).
+Proof.
+  reflexivity.
+Qed.
+
+Lemma exec_instrumented_exec_same
+      {A:         Type}
+      (w:         W)
+      (sig:       Sem.t I)
+      (p:         Program I A)
+  : execInstrumentedProgram w sig p = execProgram sig p.
+Proof.
+  revert w sig.
+  induction p.
+  + reflexivity.
+  + intros w sig.
+    rewrite execInstrumentedProgram_equation_2.
+    now rewrite H.
+Qed.
+
+Definition evalInstrumentedProgram
+           {A:         Type}
+           (w:         W)
+           (sig:       Sem.t I)
+           (p:         Program I A)
+  : A :=
+  fst (Sem.res (runInstrumentedProgram w sig p)).
+
+Lemma evalInstrumentedProgram_equation_2
+      {A B: Type}
+      (w: W)
+      (sig: Sem.t I)
+      (e: I A)
+      (f: A -> Program I B)
+  : evalInstrumentedProgram w sig (Request e f)
+    = evalInstrumentedProgram
+        (abs_step _ e (evalEffect sig e) w)
+        (execEffect sig e)
+        (f (evalEffect sig e)).
+Proof.
+  reflexivity.
+Qed.
+
+Lemma eval_instrumented_eval_same
+      {A:         Type}
+      (w:         W)
+      (sig:       Sem.t I)
+      (p:         Program I A)
+  : evalInstrumentedProgram w sig p = evalProgram sig p.
+Proof.
+  revert w sig.
+  induction p.
+  + reflexivity.
+  + intros w sig.
+    rewrite evalInstrumentedProgram_equation_2.
+    now rewrite H.
+Qed.
+
+Definition witnessInstrumentedProgram
+           {A:        Type}
+           (w:        W)
+           (sig:      Sem.t I)
+           (p:        Program I A)
+  : W :=
+  snd (Sem.res (runInstrumentedProgram w sig p)).
+
+Lemma witnessInstrumentedProgram_equation_2
+      {A B:      Type}
+      (w:        W)
+      (sig:      Sem.t I)
+      (e:        I A)
+      (f:        A -> Program I B)
+  : witnessInstrumentedProgram w sig (Request e f)
+    = witnessInstrumentedProgram
+        (abs_step _ e (evalEffect sig e) w)
+        (execEffect sig e)
+        (f (evalEffect sig e)).
+Proof.
+  reflexivity.
+Qed.
+
+Add Parametric Morphism
+    (A: Type) `{Equality A}
+  : (witnessInstrumentedProgram)
+    with signature eq ==> (@equal (Sem.t I) _) ==> (@equal (Program I A) _) ==> eq
+      as derive_abstraction_morphism.
+Proof.
+  intros w sig sig' Heq_sig p q Heq_p.
+  cbn in Heq_p; subst.
+  revert w sig sig' Heq_sig.
+  induction q.
+  + reflexivity.
+  + intros w sig sig' [Heq_1 Heq_2].
+    repeat rewrite witnessInstrumentedProgram_equation_2.
+    rewrite Heq_1.
+    apply H0.
+    apply Heq_2.
+Qed.
+End def.
+
+Arguments runInstrumentedProgram [W I] (abs_step) [A] (w sig p).
+Arguments evalInstrumentedProgram [W I] (abs_step) [A] (w sig p).
+Arguments execInstrumentedProgram [W I] (abs_step) [A] (w sig p).
+Arguments witnessInstrumentedProgram [W I] (abs_step) [A] (w sig p).
+Arguments exec_instrumented_exec_same [W I] (abs_step) [A] (w sig p).
+Arguments eval_instrumented_eval_same [W I] (abs_step) [A] (w sig p).
+
+(** * Abstract Specification
 
     An Abstract Specification allows for defining an expected
     behaviour for an [Interface] operational [Semantics]. This
@@ -40,10 +212,7 @@ Require Import FreeSpec.Abstract.
 
     These predicates are tied to an abstract state. This abstract
     state is modified by the [abstract_step] function through the
-    execution (see [abstractRun] for more information about that).
-
- *)
-
+    execution (see [abstractRun] for more information about that). *)
 Record Specification
        (W:  Type)
        (I:  Type -> Type)
@@ -58,27 +227,36 @@ Record Specification
       : I A -> A -> W -> Prop
     }.
 
-Arguments abstract_step [_ _] (_) [_] (_ _ _).
-Arguments precondition  [_ _] (_) [_] (_ _).
-Arguments postcondition [_ _] (_) [_] (_ _).
+Arguments abstract_step [W I] (_) [A] (e x w).
+Arguments precondition [W I] (_) [A] (e w).
+Arguments postcondition [W I] (_) [A] (e x w).
+
+Definition no_pre
+           {I:  Interface}
+           {W:  Type}
+           (A:  Type)
+           (e:  I A)
+           (w:  W)
+  : Prop :=
+  True.
 
 Definition specification_derive
            {W:    Type}
            {I:    Interface}
            {A:    Type}
            (p:    Program I A)
-           (sig:  Semantics I)
+           (sig:  Sem.t I)
            (c:    Specification W I)
            (w:    W)
   : W :=
-  deriveAbstraction w (abstract_step c) sig p.
+  witnessInstrumentedProgram (abstract_step c) w sig p.
 
 Fact specification_derives_pure_eq
      {W:    Type}
      {I:    Interface}
      {A:    Type}
      (x:    A)
-     (sig:  Semantics I)
+     (sig:  Sem.t I)
      (c:    Specification W I)
      (w:    W)
   : specification_derive (Pure x) sig c w = w.
@@ -87,12 +265,12 @@ Proof.
 Qed.
 
 Fact specification_derives_request_eq
-     {W:    Type}
-     {I:    Interface}
-     {A B:  Type}
+     (W:    Type)
+     (I:    Interface)
+     (A B:  Type)
      (e:    I A)
      (f:    A -> Program I B)
-     (sig:  Semantics I)
+     (sig:  Sem.t I)
      (c:    Specification W I)
      (w:    W)
   : specification_derive (Request e f) sig c w
@@ -117,21 +295,19 @@ Qed.
     executes an effect which satisfies the precondition, then the
     resulting operational Semantics complies with [c] in accordance
     with the new abstract state computed with the [abstract_step]
-    function.
-
- *)
+    function. *)
 
 CoInductive compliant_semantics
             {W:    Type}
             {I:    Interface}
             (c:    Specification W I)
             (w:    W)
-            (sig:  Semantics I)
+            (sig:  Sem.t I)
   : Prop :=
 | enforced (Hprom: forall {A:  Type}
                           (e:  I A),
                precondition c e w
-               -> (postcondition c e) (evalEffect sig e) w)
+               -> postcondition c e (evalEffect sig e) w)
            (Henf:  forall {A:  Type}
                           (e:  I A),
                precondition c e w
@@ -141,37 +317,33 @@ CoInductive compliant_semantics
   : compliant_semantics c w sig.
 
 Notation "sig '|=' c '[' w ']'" :=
-  (compliant_semantics c w sig)
-    (at level 60, no associativity).
+  (compliant_semantics c w sig) (at level 60).
 
 Corollary compliant_enforces_postcondition
-      {W:     Type}
-      {I:     Interface}
-      {A:     Type}
-      (e:     I A)
-      (sig:   Semantics I)
-      (c:     Specification W I)
-      (w:     W)
-      (Henf:  sig |= c[w])
-      (Hreq:  precondition c e w)
+          (W:     Type)
+          (I:     Interface)
+          (A:     Type)
+          (e:     I A)
+          (sig:   Sem.t I)
+          (c:     Specification W I)
+          (w:     W)
+          (Henf:  sig |= c[w])
+          (Hreq:  precondition c e w)
   : postcondition c e (evalEffect sig e) w.
 Proof.
   destruct Henf.
-  apply Hprom.
-  exact Hreq.
+  now apply Hprom.
 Qed.
 
-(** ** Compliant Stateful Semantics
-
- *)
+(** ** Compliant Stateful Semantics *)
 
 Definition specification_preserves_inv
-           {W:      Type}
-           {I:      Interface}
-           {S:      Type}
-           (c:      Specification W I)
-           (inv:    W -> S -> Prop)
-           (step:   @PS I S)
+           {W:     Type}
+           {I:     Interface}
+           {S:     Type}
+           (c:     Specification W I)
+           (inv:   W -> S -> Prop)
+           (step:  @PS I S)
   := forall (A:  Type)
             (e:  I A)
             (w:  W)
@@ -207,7 +379,7 @@ Fact _stateful_specification_enforcement
            (Henf:   specification_enforces_postcondition c inv step)
            (s:      S),
     inv w s
-    -> (mkSemantics step s) |= c[w].
+    -> mkSemantics step s |= c[w].
 Proof.
   cofix _stateful_specification_enforcement.
   intros w Hpres Henf s Hinv .
@@ -221,7 +393,7 @@ Proof.
     ++ apply  Hpres.
     ++ apply  Henf.
     ++ cbn in *.
-       apply (Hpres _ _ _ _ Hinv Hreq).
+       now eapply Hpres.
 Qed.
 
 Lemma stateful_specification_enforcement
@@ -236,7 +408,7 @@ Lemma stateful_specification_enforcement
       (Henf:  specification_enforces_postcondition c inv step)
   : forall (s: S),
     inv w s
-    -> (mkSemantics step s) |= c[w].
+    -> mkSemantics step s |= c[w].
 Proof.
   intros s Hinv.
   apply (_stateful_specification_enforcement c inv step w Hpres Henf s Hinv).
@@ -247,11 +419,9 @@ Qed.
     In a nutshell, a given [p: Program I A] is said correct with
     respect to a given abstract [Specification] [c] if, given a
     semantics for [I] which complies with [c] in accordance with [w:
-    W], [p] only uses effects which satisfy the precondition.
+    W], [p] only uses effects which satisfy the precondition. *)
 
-    ** Definition
-
- *)
+(** ** Definition *)
 
 Inductive correct_program
           {W:  Type}
@@ -266,230 +436,35 @@ Inductive correct_program
                     (e:     I A)
                     (f:     A -> Program I B)
                     (Hreq:  precondition c e w)
-                    (Hnext:  forall (sig: Semantics I)
+                    (Hnext:  forall (sig: Sem.t I)
                                     (Henf: sig |= c[w]),
                         correct_program c
                                         (abstract_step c e (evalEffect sig e) w)
                                         (f (evalEffect sig e)))
   : correct_program c w (Request e f).
 
-Notation "p '=|' c '[' w ']'" :=
+Notation "p '|>' c '[' w ']'" :=
   (correct_program c w p)
     (at level 59, no associativity).
 
-(** ** Compliance Preservation
-
-    In order to prove the [compliance_correct_compliance] lemmas, we
-    first highlight several convenient properties of
-    [compliant_semantics] and [correct_program].
-
- *)
-
-Fact pure_compliant_semantics
-     {W:    Type}
-     {I:    Interface}
-     {A:    Type}
-     (x:    A)
-     (sig:  Semantics I)
-     (c:    Specification W I)
-     (w:    W)
-     (H:    sig |= c[w])
-  : abstractExec w (abstract_step c) sig (Pure x)
-      |= c[specification_derive (Pure x) sig c w].
-Proof.
-  rewrite (specification_derives_pure_eq x sig c).
-  exact H.
-Qed.
-
-Fact specification_derive_assoc
-     {W:      Type}
-     {I:      Interface}
-     {A B C:  Type}
-     (p:      Program I A)
-     (f:      A -> Program I B)
-     (g:      B -> Program I C)
-     (sig:    Semantics I)
-     (c:      Specification W I)
-     (w:      W)
-  : specification_derive (pbind (pbind p f) g) sig c w
-    = specification_derive (pbind p (fun x => pbind (f x) g)) sig c w.
-Proof.
-  rewrite program_eq_bind_assoc.
-  reflexivity.
-Qed.
-
-Fact exec_abs_assoc
-     {W:  Type}
-     {I:  Interface}
-     {A:  Type}
-     (p:  Program I A)
-  : forall {B:    Type}
-           (f:    A -> Program I B)
-           (sig:  Semantics I)
-           (c:    Specification W I)
-           (w:    W),
-    abstractExec w (abstract_step c) sig (pbind p f)
-    = abstractExec (specification_derive p sig c w)
-                   (abstract_step c)
-                   (abstractExec w (abstract_step c) sig p)
-                   (f (evalProgram sig p)).
-Proof.
-  intros B f sig c s.
-  repeat rewrite abstract_exec_exec_program_same.
-  revert sig; induction p; [reflexivity |]; intros sig.
-  apply H.
-Qed.
-
-Fact eval_program_assoc
-     {W:  Type}
-     {I:  Interface}
-     {A:  Type}
-     (p:  Program I A)
-  : forall {B:    Type}
-           (f:    A -> Program I B)
-           (sig:  Semantics I)
-           (c:    Specification W I)
-           (w:    W),
-    evalProgram sig (pbind p f)
-    = evalProgram (abstractExec w (abstract_step c) sig p)
-                  (f (evalProgram sig p)).
-Proof.
-  intros B f sig c s.
-  rewrite abstract_exec_exec_program_same.
-  revert sig; induction p; [reflexivity |]; intros sig.
-  apply H.
-Qed.
-
-Fact specification_derive_bind
-     {W:  Type}
-     {I:  Interface}
-     {A:  Type}
-     (p:  Program I A)
-  : forall {B:    Type}
-           (f:    A -> Program I B)
-           (sig:  Semantics I)
-           (c:    Specification W I)
-           (w:    W),
-    specification_derive (f (evalProgram sig p))
-                         (abstractExec w (abstract_step c) sig p)
-                         c
-                         (specification_derive p sig c w)
-    = specification_derive (pbind p f) sig c w.
-Proof.
-  induction p.
-  + reflexivity.
-  + intros C f' sig' c' w'.
-    apply H.
-Qed.
-
-Fact abstractExec_Bind
-     {W:    Type}
-     {I:    Interface}
-     {A B:  Type}
-     (p:    Program I A)
-  : forall (f:    A -> Program I B)
-           (sig:  Semantics I)
-           (c:    Specification W I)
-           (w:    W),
-    abstractExec (specification_derive p sig c w)
-                 (abstract_step c)
-                 (abstractExec w
-                               (abstract_step c)
-                               sig
-                               p)
-                 (f (evalProgram sig p))
-    = abstractExec w (abstract_step c) sig (pbind p f).
-Proof.
-  intros f sig c w.
-  repeat rewrite abstract_exec_exec_program_same.
-  rewrite exec_program_bind_assoc.
-  reflexivity.
-Qed.
-
-Lemma compliant_correct_compliant
+Lemma correct_program_compliant_semantics_compliant_semantics
       {W:  Type}
       {I:  Interface}
       {A:  Type}
-      (p:  Program I A)
-  : forall (c:    Specification W I)
-           (w:    W)
-           (sig:  Semantics I)
-           (H:    sig |= c[w])
-           (Hp:   p =| c[w]),
-    (abstractExec w (abstract_step c) sig p) |= c[specification_derive p sig c w].
+      (c:  Specification W I)
+      (w:  W)
+      (sig: Sem.t I)
+      (p: Program I A)
+  : sig |= c[w]
+    -> p |> c[w]
+    -> execProgram sig p |= c[specification_derive p sig c w].
 Proof.
-  induction p.
-  + intros c w sig He Hp;
-      apply (pure_compliant_semantics a sig c w He).
-  + intros c w sig He Hp.
-    constructor.
-    ++ apply H;
-         dependent induction Hp.
-         +++ now apply He.
-         +++ now apply Hnext.
-    ++ apply H;
-         dependent induction Hp.
-       +++ now apply He in Hreq.
-       +++ now apply Hnext.
-Qed.
-
-Lemma correct_pbind_correct_left_operand
-      {W:    Type}
-      {I:    Interface}
-      {A B:  Type}
-      (w:    W)
-      (c:    Specification W I)
-      (p:    Program I A)
-      (f:    A -> Program I B)
-  : pbind p f =| c[w]
-    -> p =| c[w].
-Proof.
-  revert w; induction p; intro w.
-  + intro.
-    constructor.
-  + cbn.
-    constructor.
-    ++ dependent induction H0.
-       apply Hreq.
-    ++ intros sig Hsig.
-       apply H.
-       dependent induction H0.
-       now apply Hnext.
-Qed.
-
-Lemma correct_bind_correct_right_operand
-      {W:     Type}
-      {I:     Interface}
-      {A B:   Type}
-      (w:     W)
-      (c:     Specification W I)
-      (p:     Program I A)
-      (f:     A -> Program I B)
-      (sig:   Semantics I)
-      (Hsig:  sig |= c[w])
-  : pbind p f =| c[w]
-    -> f (evalProgram sig p) =| c [specification_derive p sig c w].
-Proof.
-  revert Hsig;
-    revert sig;
-    revert w;
-    induction p;
-    intros w sig Hsig.
+  intros Hsig Hp.
+  revert sig Hsig.
+  induction Hp.
   + auto.
-  + cbn.
-    intro Hc.
-    apply H.
-    apply Hsig.
-    ++ now dependent induction Hc.
-    ++ dependent induction Hc.
-       now apply Hnext.
+  + intros sig Hsig.
+    apply (H sig Hsig).
+    destruct Hsig.
+    now apply Henf.
 Qed.
-
-Definition no_pre
-           {I:  Interface}
-           {W:  Type}
-           (A:  Type)
-           (e:  I A)
-           (w:  W)
-  : Prop :=
-  True.
