docs/core.scrbl
@@ -1,0 +1,8 @@
+#lang scribble/manual
+@(require "macros.scrbl")
+
+@title{FreeSpec.Core}
+
+@include-section{core/specifying.scrbl}
+@include-section{core/verifying.scrbl}
+@include-section{core/composing.scrbl}
