docs/core/verifying.scrbl
@@ -1,0 +1,5 @@
+#lang scribble/manual
+
+@(require "../macros.scrbl")
+
+@title{Verifying Components}
