docs/exec.scrbl
@@ -1,0 +1,7 @@
+#lang scribble/manual
+@(require "macros.scrbl")
+
+@title{FreeSpec.Exec}
+
+@include-section{exec/interfaces.scrbl}
+@include-section{exec/exec.scrbl}
