docs/exec/exec.scrbl
@@ -1,0 +1,4 @@
+#lang scribble/manual
+@(require "../macros.scrbl")
+
+@title{The @code{Exec} Command}
