docs/exec/interfaces.scrbl
@@ -1,0 +1,10 @@
+#lang scribble/manual
+@(require "../macros.scrbl")
+
+@title{Supported Interfaces}
+
+@section{@code{Console.i}}
+
+@subsection{@code{scan}}
+
+@subsection{@code{echo}}
