docs/macros.scrbl
@@ -1,0 +1,7 @@
+#lang scribble/base
+
+@(define -> "→")
+@(define forall "∀")
+@(define sigma "σ")
+
+@(provide (all-defined-out))
